src/SDK/AwsEncryptionSdk.dfy
@@ -1,0 +1,39 @@
+// Copyright Amazon.com Inc. or its affiliates. All Rights Reserved.
+// SPDX-License-Identifier: Apache-2.0
+
+include "../StandardLibrary/StandardLibrary.dfy"
+include "../StandardLibrary/UInt.dfy"
+include "../Generated/AwsCryptographicMaterialProviders.dfy"
+include "../Generated/AwsEncryptionSdk.dfy"
+include "../Util/UTF8.dfy"
+include "EncryptDecrypt.dfy"
+
+module {:extern "AwsEncryptionSdk"} AwsEncryptionSdk {
+  import opened Wrappers
+  import opened StandardLibrary
+  import opened UInt = StandardLibrary.UInt
+  import UTF8
+  import Aws.Crypto
+  import Aws.Esdk
+  import EncryptDecrypt
+
+  // move to different module
+  class AwsEncryptionSdkClient extends Esdk.IAwsEncryptionSdkClient {
+        constructor () {}
+
+        method Encrypt(input: Esdk.EncryptInput) returns (res: Result<Esdk.EncryptOutput, string>)
+            requires input.Valid()
+        {
+            var encryptRequest := EncryptDecrypt.EncryptRequest.WithCMM(input.plaintext, input.materialsManager).SetEncryptionContext(input.encryptionContext);
+            var e :- expect EncryptDecrypt.Encrypt(encryptRequest);
+            return Success(Esdk.EncryptOutput(ciphertext:=e));
+        }
+        method Decrypt(input: Esdk.DecryptInput) returns (res: Result<Esdk.DecryptOutput, string>)
+            requires input.Valid()
+        {
+            var decryptRequest := EncryptDecrypt.DecryptRequest.WithCMM(input.ciphertext, input.materialsManager);
+            var d :- expect EncryptDecrypt.Decrypt(decryptRequest);
+            return Success(Esdk.DecryptOutput(plaintext:=d));
+        }
+  }
+}
