src/SDK/Deserialize.dfy
@@ -9,7 +9,6 @@ include "AlgorithmSuite.dfy"
 include "../Util/Streams.dfy"
 include "../StandardLibrary/StandardLibrary.dfy"
 include "../Util/UTF8.dfy"
-include "../Generated/AwsCryptographicMaterialProviders.dfy"
 
 /*
  * The message header deserialization
@@ -90,9 +89,15 @@ module Deserialize {
     var _ :- DeserializeReserved(rd);
     ghost var reserveEnd := rd.reader.pos;
 
+    // TODO dafny verification handholding
+    assert [version as uint8] + [typ as uint8] + UInt16ToSeq(algorithmSuiteID as uint16) + messageID + rd.reader.data[aadStart..aadEnd]
+      + Msg.EDKsToSeq(encryptedDataKeys) + [Msg.ContentTypeToUInt8(contentType)] + [0,0,0,0]  ==
+      rd.reader.data[old(rd.reader.pos)..rd.reader.pos];
+
     var ivLength :- rd.ReadByte();
     var frameLength :- rd.ReadUInt32();
 
+    // TODO dafny verification handholding
     assert [version as uint8] + [typ as uint8] + UInt16ToSeq(algorithmSuiteID as uint16) + messageID + rd.reader.data[aadStart..aadEnd]
       + Msg.EDKsToSeq(encryptedDataKeys) + [Msg.ContentTypeToUInt8(contentType)] + [0,0,0,0] + [ivLength] + UInt32ToSeq(frameLength) ==
       rd.reader.data[old(rd.reader.pos)..rd.reader.pos];
