test/SDK/Keyring/RawAESKeyring.dfy
@@ -1,7 +1,7 @@
 // Copyright Amazon.com Inc. or its affiliates. All Rights Reserved.
 // SPDX-License-Identifier: Apache-2.0
 
-include "../../../src/SDK/Keyring/PolymorphRawAESKeyring.dfy"
+include "../../../src/SDK/Keyring/RawAESKeyring.dfy"
 include "../../../src/SDK/AlgorithmSuite.dfy"
 include "../../../src/SDK/MessageHeader.dfy"
 include "../../../src/SDK/Materials.dfy"
@@ -14,11 +14,11 @@ include "../../../src/Util/UTF8.dfy"
 include "../../../src/Generated/AwsCryptographicMaterialProviders.dfy"
 include "../../Util/TestUtils.dfy"
 
-module TestPolymorphAESKeyring {
+module TestAESKeyring {
   import opened Wrappers
   import opened UInt = StandardLibrary.UInt
   import AESEncryption
-  import PolymorphRawAESKeyringDef
+  import RawAESKeyringDef
   import MessageHeader
   import Materials
   import EncryptionContext
@@ -31,7 +31,7 @@ module TestPolymorphAESKeyring {
   method {:test} TestOnEncryptOnDecryptGenerateDataKey()
   {
     var namespace, name := TestUtils.NamespaceAndName(0);
-    var rawAESKeyring := new PolymorphRawAESKeyringDef.PolymorphRawAESKeyring(namespace, name, seq(32, i => 0), EncryptionSuites.AES_GCM_256);
+    var rawAESKeyring := new RawAESKeyringDef.RawAESKeyring(namespace, name, seq(32, i => 0), EncryptionSuites.AES_GCM_256);
     var encryptionContext := TestUtils.SmallEncryptionContext(TestUtils.SmallEncryptionContextVariation.A);
     ExpectSerializableEncryptionContext(encryptionContext);
 
@@ -81,7 +81,7 @@ module TestPolymorphAESKeyring {
   method {:test} TestOnEncryptOnDecryptSuppliedDataKey()
   {
     var namespace, name := TestUtils.NamespaceAndName(0);
-    var rawAESKeyring := new PolymorphRawAESKeyringDef.PolymorphRawAESKeyring(namespace, name, seq(32, i => 0), EncryptionSuites.AES_GCM_256);
+    var rawAESKeyring := new RawAESKeyringDef.RawAESKeyring(namespace, name, seq(32, i => 0), EncryptionSuites.AES_GCM_256);
     var encryptionContext := TestUtils.SmallEncryptionContext(TestUtils.SmallEncryptionContextVariation.A);
     ExpectSerializableEncryptionContext(encryptionContext);
 
@@ -121,10 +121,10 @@ module TestPolymorphAESKeyring {
     method {:test} TestOnDecryptKeyNameMismatch()
   {
     var namespace, name := TestUtils.NamespaceAndName(0);
-    var rawAESKeyring := new PolymorphRawAESKeyringDef.PolymorphRawAESKeyring(namespace, name, seq(32, i => 0), EncryptionSuites.AES_GCM_256);
+    var rawAESKeyring := new RawAESKeyringDef.RawAESKeyring(namespace, name, seq(32, i => 0), EncryptionSuites.AES_GCM_256);
 
     var mismatchName :- expect UTF8.Encode("mismatched");
-    var mismatchedAESKeyring := new PolymorphRawAESKeyringDef.PolymorphRawAESKeyring(namespace, mismatchName, seq(32, i => 0), EncryptionSuites.AES_GCM_256);
+    var mismatchedAESKeyring := new RawAESKeyringDef.RawAESKeyring(namespace, mismatchName, seq(32, i => 0), EncryptionSuites.AES_GCM_256);
 
     var encryptionContext := TestUtils.SmallEncryptionContext(TestUtils.SmallEncryptionContextVariation.A);
     ExpectSerializableEncryptionContext(encryptionContext);
@@ -171,7 +171,7 @@ module TestPolymorphAESKeyring {
   method {:test} TestOnDecryptNoEDKs()
   {
     var namespace, name := TestUtils.NamespaceAndName(0);
-    var rawAESKeyring := new PolymorphRawAESKeyringDef.PolymorphRawAESKeyring(namespace, name, seq(32, i => 0), EncryptionSuites.AES_GCM_256);
+    var rawAESKeyring := new RawAESKeyringDef.RawAESKeyring(namespace, name, seq(32, i => 0), EncryptionSuites.AES_GCM_256);
     var wrappingAlgorithmID := Crypto.ALG_AES_256_GCM_IV12_TAG16_HKDF_SHA384_ECDSA_P384;
     var encryptionContext := TestUtils.SmallEncryptionContext(TestUtils.SmallEncryptionContextVariation.A);
     var verificationKey := seq(32, i => 0);
@@ -196,7 +196,7 @@ module TestPolymorphAESKeyring {
   method {:test} TestOnEncryptUnserializableEC()
   {
     var namespace, name := TestUtils.NamespaceAndName(0);
-    var rawAESKeyring := new PolymorphRawAESKeyringDef.PolymorphRawAESKeyring(namespace, name, seq(32, i => 0), EncryptionSuites.AES_GCM_256);
+    var rawAESKeyring := new RawAESKeyringDef.RawAESKeyring(namespace, name, seq(32, i => 0), EncryptionSuites.AES_GCM_256);
     var unserializableEncryptionContext := generateUnserializableEncryptionContext();
     ExpectNonSerializableEncryptionContext(unserializableEncryptionContext);
 
@@ -225,7 +225,7 @@ module TestPolymorphAESKeyring {
     // Set up valid EDK for decryption
     var encryptionContext := TestUtils.SmallEncryptionContext(TestUtils.SmallEncryptionContextVariation.A);
     var namespace, name := TestUtils.NamespaceAndName(0);
-    var rawAESKeyring := new PolymorphRawAESKeyringDef.PolymorphRawAESKeyring(namespace, name, seq(32, i => 0), EncryptionSuites.AES_GCM_256);
+    var rawAESKeyring := new RawAESKeyringDef.RawAESKeyring(namespace, name, seq(32, i => 0), EncryptionSuites.AES_GCM_256);
     var wrappingAlgorithmID := Crypto.ALG_AES_256_GCM_IV12_TAG16_HKDF_SHA384_ECDSA_P384;
     var signingKey := seq(32, i => 0);
     var encryptionMaterialsIn := Crypto.EncryptionMaterials(
@@ -259,7 +259,7 @@ module TestPolymorphAESKeyring {
     var ciphertext := [0, 1, 2, 3];
     var authTag := [4, 5, 6, 7];
     var serializedEDKCiphertext := ciphertext + authTag;
-    var encOutput := PolymorphRawAESKeyringDef.DeserializeEDKCiphertext(serializedEDKCiphertext, |authTag|);
+    var encOutput := RawAESKeyringDef.DeserializeEDKCiphertext(serializedEDKCiphertext, |authTag|);
 
     expect encOutput.cipherText == ciphertext;
     expect encOutput.authTag == authTag;
@@ -269,7 +269,7 @@ module TestPolymorphAESKeyring {
     var ciphertext := [0, 1, 2, 3];
     var authTag := [4, 5, 6, 7];
     var encOutput := AESEncryption.EncryptionOutput(ciphertext, authTag);
-    var serializedEDKCiphertext := PolymorphRawAESKeyringDef.SerializeEDKCiphertext(encOutput);
+    var serializedEDKCiphertext := RawAESKeyringDef.SerializeEDKCiphertext(encOutput);
 
     expect serializedEDKCiphertext == ciphertext + authTag;
   }
